library/data/dlist.lean
@@ -22,8 +22,7 @@ variables {α : Type u}
 local notation `♯`:max := by abstract { intros, simp }
 
 /-- Convert a list to a dlist -/
-def of_list (l : list α) : dlist α :=
-⟨append l, ♯⟩
+def of_list (l : list α) : dlist α := ⟨concat l, ♯⟩
 
 /-- Convert a lazily-evaluated list to a dlist -/
 def lazy_of_list (l : thunk (list α)) : dlist α :=
@@ -50,17 +49,16 @@ def cons (x : α) : dlist α →  dlist α
 | ⟨xs, h⟩ := ⟨x::_ ∘ xs, by abstract { intros, simp, rw [←h] }⟩
 
 /-- `O(1)` Append a single element to a dlist -/
-def concat (x : α) : dlist α → dlist α
+def append (x : α) : dlist α → dlist α
 | ⟨xs, h⟩ := ⟨xs ∘ x::_, by abstract { intros, simp, rw [h, h [x]], simp }⟩
 
-/-- `O(1)` Append dlists -/
-protected def append : dlist α → dlist α → dlist α
+/-- `O(1)` Concatenate dlists -/
+protected def concat : dlist α → dlist α → dlist α
 | ⟨xs, h₁⟩ ⟨ys, h₂⟩ := ⟨xs ∘ ys, by { intros, simp, rw [h₂, h₁, h₁ (ys list.nil)], simp } ⟩
 
-instance : has_append (dlist α) :=
-⟨dlist.append⟩
+instance : has_concat (dlist α) := ⟨dlist.concat⟩
 
-local attribute [simp] of_list to_list empty singleton cons concat dlist.append
+local attribute [simp] of_list to_list empty singleton cons concat dlist.concat
 
 lemma to_list_of_list (l : list α) : to_list (of_list l) = l :=
 by cases l; simp
@@ -68,7 +66,7 @@ by cases l; simp
 lemma of_list_to_list (l : dlist α) : of_list (to_list l) = l :=
 begin
    cases l with xs,
-   have h : append (xs []) = xs,
+   have h : concat (xs []) = xs,
    { intros, funext x, simp [l_invariant x] },
    simp [h]
 end
@@ -79,14 +77,14 @@ by simp
 lemma to_list_singleton (x : α) : to_list (singleton x) = [x] :=
 by simp
 
-lemma to_list_append (l₁ l₂ : dlist α) : to_list (l₁ ++ l₂) = to_list l₁ ++ to_list l₂ :=
-show to_list (dlist.append l₁ l₂) = to_list l₁ ++ to_list l₂, from
+lemma to_list_concat (l₁ l₂ : dlist α) : to_list (l₁ ++ l₂) = to_list l₁ ++ to_list l₂ :=
+show to_list (dlist.concat l₁ l₂) = to_list l₁ ++ to_list l₂, from
 by cases l₁; cases l₂; simp; rw l₁_invariant
 
 lemma to_list_cons (x : α) (l : dlist α) : to_list (cons x l) = x :: to_list l :=
 by cases l; simp
 
-lemma to_list_concat (x : α) (l : dlist α) : to_list (concat x l) = to_list l ++ [x] :=
+lemma to_list_append (x : α) (l : dlist α) : to_list (append x l) = to_list l ++ [x] :=
 by cases l; simp; rw [l_invariant]
 
 end dlist
