tests/lean/run/regset.lean
@@ -7,7 +7,7 @@ parameter symbol : Type
 set (list symbol)
 
 def concat : lang → lang → lang :=
-λ a b : lang, { ll : list symbol | ∃xs ys : list symbol, ll = list.append xs ys ∧ xs ∈ a ∧ ys ∈ b }
+λ a b : lang, { ll : list symbol | ∃xs ys : list symbol, ll = list.concat xs ys ∧ xs ∈ a ∧ ys ∈ b }
 
 end
 end regset
