tests/lean/run/back3.lean
@@ -5,8 +5,8 @@ open list tactic
 universe variable u
 lemma in_tail  {α : Type u} {a : α} (b : α) {l : list α}        : a ∈ l → a ∈ b::l   := mem_cons_of_mem _
 lemma in_head  {α : Type u} (a : α) (l : list α)                : a ∈ a::l           := mem_cons_self _ _
-lemma in_left  {α : Type u} {a : α}   {l : list α} (r : list α) : a ∈ l → a ∈ l ++ r := mem_append_left _
-lemma in_right {α : Type u} {a : α}   (l : list α) {r : list α} : a ∈ r → a ∈ l ++ r := mem_append_right _
+lemma in_left  {α : Type u} {a : α}   {l : list α} (r : list α) : a ∈ l → a ∈ l ++ r := mem_concat_left _
+lemma in_right {α : Type u} {a : α}   (l : list α) {r : list α} : a ∈ r → a ∈ l ++ r := mem_concat_right _
 
 /- It is trivial to define mk_mem_list using backward chaining -/
 attribute [intro] in_tail in_head in_left in_right
