tests/lean/run/ind_issue.lean
@@ -1,9 +1,9 @@
 def stack := list nat
-instance : has_append stack :=
+instance : has_concat stack :=
 by unfold stack; apply_instance
 
 example (s : stack) : s ++ [] = s :=
 begin
   induction s,
-  refl, apply list.append_nil
+  refl, apply list.concat_nil
 end
