tests/lean/run/listex.lean
@@ -11,9 +11,9 @@ meta def search_mem_list : expr → expr → tactic expr
 | a e :=
 (do m ← mk_app ``has_mem.mem [a, e], find_assumption m)
 <|>
-(do [_, _, l, r] ← match_app_of e ``has_append.append | failed, h ← search_mem_list a l, mk_app `in_left [l, r, h])
+(do [_, _, l, r] ← match_app_of e ``has_concat.concat | failed, h ← search_mem_list a l, mk_app `in_left [l, r, h])
 <|>
-(do [_, _, l, r] ← match_app_of e ``has_append.append | failed, h ← search_mem_list a r, mk_app `in_right [l, r, h])
+(do [_, _, l, r] ← match_app_of e ``has_concat.concat | failed, h ← search_mem_list a r, mk_app `in_right [l, r, h])
 <|>
 (do [_, b, t] ← match_app_of e ``list.cons | failed, is_def_eq a b, mk_app `in_head [b, t])
 <|>
